theories/Algorithmic/Typing/Lemmas.v
@@ -7,13 +7,6 @@ From McPTS.Core.Semantic Require Import Consequences.
 From McPTS.Frontend Require Import Elaborator.
 Import Domain_Notations.
 
-Record FunctionalSig (P : PtsSig) : Prop :=
-  mkFunctionalSig {
-      Func_ax_typ : forall s1 s2 s2', Ax_typ P s1 s2 -> Ax_typ P s1 s2' -> s2 = s2';
-      Func_ru_pi : forall s1 s2 s3 s3', Ru_pi P s1 s2 s3 -> Ru_pi P s1 s2 s3' -> s3 = s3';
-      Func_ru_nat : forall s s', Ru_nat P s -> Ru_nat P s' -> s = s';
-    }.
-
 Lemma functional_alg_type_infer {P} (pred_P : PredicativeSig P) (func_P : FunctionalSig P) : forall {Γ : ctx P} {A A' M},
     {{ Γ ⊢a M ⟹ A }} ->
     {{ Γ ⊢a M ⟹ A' }} ->
