theories/CaseStudies/MiniML/Entrypoint.v
@@ -3,28 +3,28 @@ From Coq Require Import ExtrOcamlBasic ExtrOcamlNatInt ExtrOcamlNativeString Ext
 
 From Equations Require Import Equations.
 
-From McPTS Require Import LibTactics.
+From McPTS Require Import PtsSignature LibTactics.
 From McPTS.Core Require Import Base Completeness Soundness.
 From McPTS.Core.Syntactic Require Import SystemOpt.
 From McPTS.Extraction Require Import NbE TypeCheck.
-From McPTS.CaseStudies.MiniML Require Import Parser.
+From McPTS.CaseStudies.MiniML Require Import Signature Frontend Parser.
 Import MenhirLibParser.Inter.
 Import Syntax_Notations.
 
 Variant main_result :=
   | AllGood : forall cst_typ cst_exp A M W,
-      elaborate cst_typ nil = Some A ->
-      elaborate cst_exp nil = Some M ->
+      elaborate' cst_typ nil = Some A ->
+      elaborate' cst_exp nil = Some M ->
       {{ ⋅ ⊢ M : A }} ->
       nbe {{{ ⋅ }}} M A W ->
       main_result
-  | TypeCheckingFailure : forall A M, ~ {{ ⋅ ⊢ M : A }} -> main_result
-  | ElaborationFailure : forall cst, elaborate cst nil = None -> main_result
+  | TypeCheckingFailure : forall (A : typ MiniML_Sig) M, ~ {{ ⋅ ⊢ M : A }} -> main_result
+  | ElaborationFailure : forall cst, elaborate' cst nil = None -> main_result
   | ParserFailure : Aut.state -> Aut.Gram.token -> main_result
   | ParserTimeout : nat -> main_result
 .
 
-Definition inspect {A} (x : A) : { y | x = y } := exist _ x eq_refl.
+Definition inspect {A} (x : A) : { y | x = y } := exist _ x (eq_refl _).
 Extraction Inline inspect.
 
 #[local]
@@ -32,9 +32,9 @@ Ltac impl_obl_tac := try eassumption.
 #[tactic="impl_obl_tac"]
 Equations main (log_fuel : nat) (buf : buffer) : main_result :=
 | log_fuel, buf with Parser.prog log_fuel buf => {
-  | Parsed_pr (cst_exp, cst_typ) _ with inspect (elaborate cst_typ nil) => {
-    | exist _ (Some A) _ with inspect (elaborate cst_exp nil) => {
-      | exist _ (Some M) _ with type_check_closed A _ M _ => {
+  | Parsed_pr (cst_exp, cst_typ) _ with inspect (elaborate' cst_typ nil) => {
+    | exist _ (Some A) _ with inspect (elaborate' cst_exp nil) => {
+      | exist _ (Some M) _ with type_check_closed MiniML_Decidable MiniML_Predicative MiniML_Functional A _ M _ => {
         | left  _ with nbe_impl {{{ ⋅ }}} M A _ => {
           | exist _ W _ => AllGood cst_typ cst_exp A M W _ _ _ _
           }
@@ -58,9 +58,10 @@ Next Obligation.
   (on_all_hyp: fun H => apply soundness in H as [? []]).
   eapply nbe_order_sound.
   eassumption.
+  eapply MiniML_Predicative.
 Qed.
 
 Extraction Language OCaml.
 
 Set Extraction Flag 1007.
-Set Extraction Output Directory "../driver/extracted".
+Set Extraction Output Directory "driver/extracted".
