theories/Core/Soundness/NatCases.v
@@ -65,7 +65,7 @@ Qed.
 (*   eauto using var_glu_elem_bot_unsorted. *)
 (* Qed. *)
 Corollary var0_glu_elem_unsorted {P} (pred_P : PredicativeSig P) : forall {a typ_rel exp_rel Γ A},
-    {{ DG a ∈ glu_typ_elem pred_P None ↘ typ_rel ↘ exp_rel }} ->
+    {{ DG a ∈ glu_typ_elem pred_P so_None ↘ typ_rel ↘ exp_rel }} ->
     {{ Γ ⊢ A ® typ_rel }} ->
     {{ Γ, A ⊢ #0 : A[Wk] ® ⇑! a (length Γ) ∈ exp_rel }}.
 Proof.
@@ -77,7 +77,7 @@ Qed.
 
 Lemma glu_rel_exp_nat {P} (pred_P : PredicativeSig P) : forall {anns Γ s} {r : Ru_nat P s},
     {{ ⟪ pred_P ⟫ ⊩ Γ with anns }} ->
-    {{ ⟪ pred_P ⟫ Γ with anns ⊩u ℕ : Sort@s @ ^None }}.
+    {{ ⟪ pred_P ⟫ Γ with anns ⊩u ℕ : Sort@s @ ^so_None }}.
 Proof.
   intros * ? [Sb].
   assert {{ ⊢ Γ }} by mauto 2.
@@ -100,13 +100,13 @@ Hint Resolve glu_rel_exp_nat : mcpts.
 
 Lemma glu_rel_exp_sub_nat {P} (pred_P : PredicativeSig P) : forall {anns Γ σ anns' Δ M s} {r : Ru_nat P s},
     {{ ⟪ pred_P ⟫ Γ with anns ⊩s σ : Δ with anns' }} ->
-    {{ ⟪ pred_P ⟫ Δ with anns' ⊩u M : ℕ @ ^(Some s) }} ->
-    {{ ⟪ pred_P ⟫ Γ with anns ⊩u M[σ] : ℕ @ ^(Some s) }}.
+    {{ ⟪ pred_P ⟫ Δ with anns' ⊩u M : ℕ @ ^(so_Some s) }} ->
+    {{ ⟪ pred_P ⟫ Γ with anns ⊩u M[σ] : ℕ @ ^(so_Some s) }}.
 Proof.
   intros.
   assert {{ Γ ⊢s σ : Δ }} by mauto 3.
   assert {{ Γ ⊢ ℕ[σ] ≈ ℕ : Sort@s }} by (econstructor; mauto 2).
-  assert {{ ⟪ pred_P ⟫ Γ with anns ⊩u M[σ] : ℕ[σ] @ ^(Some s) }} as [Sb [HgluΓ]]%glu_rel_exp_unsorted_implies_glu_rel_exp by (eapply TermStructureCases.glu_rel_exp_sub_typ_unsorted; mauto 3).
+  assert {{ ⟪ pred_P ⟫ Γ with anns ⊩u M[σ] : ℕ[σ] @ ^(so_Some s) }} as [Sb [HgluΓ]]%glu_rel_exp_unsorted_implies_glu_rel_exp by (eapply TermStructureCases.glu_rel_exp_sub_typ_unsorted; mauto 3).
   exists Sb.
   split; [eassumption |].
   intros.
@@ -125,7 +125,7 @@ Hint Resolve glu_rel_exp_sub_nat : mcpts.
 Lemma glu_rel_exp_of_nat {P} (pred_P : PredicativeSig P) : forall {s} {r : Ru_nat P s} {anns Γ Sb M},
     {{ EG Γ ∈ glu_ctx_env pred_P anns ↘ Sb }} ->
     (forall Δ σ ρ, {{ Δ ⊢s σ ® ρ ∈ Sb }} -> exists m, {{ ⟦ M ⟧ ρ ↘ m }} /\ glu_nat r Δ {{{ M[σ] }}} m) ->
-    {{ ⟪ pred_P ⟫ Γ with anns ⊩u M : ℕ @ ^(Some s) }}.
+    {{ ⟪ pred_P ⟫ Γ with anns ⊩u M : ℕ @ ^(so_Some s) }}.
 Proof.
   intros * ? Hbody.
   eexists; split; mauto 3.
@@ -140,7 +140,7 @@ Qed.
 
 Lemma glu_rel_exp_zero {P} (pred_P : PredicativeSig P) : forall {s} {r : Ru_nat P s} {anns Γ},
     {{ ⟪ pred_P ⟫ ⊩ Γ with anns }} ->
-    {{ ⟪ pred_P ⟫ Γ with anns ⊩u zero : ℕ @ ^(Some s) }}.
+    {{ ⟪ pred_P ⟫ Γ with anns ⊩u zero : ℕ @ ^(so_Some s) }}.
 Proof.
   intros * ? * [Sb].
   eapply glu_rel_exp_of_nat with (r := r); mauto 3.
@@ -152,8 +152,8 @@ Qed.
 Hint Resolve glu_rel_exp_zero : mcpts.
 
 Lemma glu_rel_exp_succ {P} (pred_P : PredicativeSig P) : forall {s} {r : Ru_nat P s} {anns Γ M},
-    {{ ⟪ pred_P ⟫ Γ with anns ⊩u M : ℕ @ ^(Some s) }} ->
-    {{ ⟪ pred_P ⟫ Γ with anns ⊩u succ M : ℕ @ ^(Some s) }}.
+    {{ ⟪ pred_P ⟫ Γ with anns ⊩u M : ℕ @ ^(so_Some s) }} ->
+    {{ ⟪ pred_P ⟫ Γ with anns ⊩u succ M : ℕ @ ^(so_Some s) }}.
 Proof.
   intros * ? * HM.
   assert {{ ⟪ pred_P ⟫ ⊩ Γ with anns }} as [SbΓ] by mauto 3.
@@ -177,16 +177,16 @@ Hint Resolve glu_rel_exp_succ : mcpts.
 
 Lemma glu_rel_sub_extend_nat {P} (pred_P : PredicativeSig P) : forall {s} {r : Ru_nat P s} {anns Γ σ anns' Δ M},
     {{ ⟪ pred_P ⟫ Γ with anns ⊩s σ : Δ with anns' }} ->
-    {{ ⟪ pred_P ⟫ Γ with anns ⊩u M : ℕ @ ^(Some s) }} ->
-    {{ ⟪ pred_P ⟫ Γ with anns ⊩s σ,,M : Δ, ℕ with (Some s)::anns' }}.
+    {{ ⟪ pred_P ⟫ Γ with anns ⊩u M : ℕ @ ^(so_Some s) }} ->
+    {{ ⟪ pred_P ⟫ Γ with anns ⊩s σ,,M : Δ, ℕ with (so_Some s)::anns' }}.
 Proof.
   intros.
   assert {{ ⟪ pred_P ⟫ ⊩ Δ with anns' }} by mauto 2.
-  assert {{ ⟪ pred_P ⟫ Γ with anns ⊩u ℕ[σ] : Sort@s @ ^None }} by mauto 3.
+  assert {{ ⟪ pred_P ⟫ Γ with anns ⊩u ℕ[σ] : Sort@s @ ^so_None }} by mauto 3.
   assert {{ Γ ⊢s σ : Δ }} by mauto 3.
   assert {{ Γ ⊢ ℕ ≈ ℕ[σ] : Sort@s }} by (symmetry; econstructor; mauto 2).
-  assert {{ ⟪ pred_P ⟫ Γ with anns ⊩u M : ℕ[σ] @ ^(Some s) }} by (eapply glu_rel_exp_conv_unsorted; mauto 3).
-  assert {{ ⟪ pred_P ⟫ Δ with anns' ⊩u ℕ : Sort@s @ ^None }} by mauto 3.
+  assert {{ ⟪ pred_P ⟫ Γ with anns ⊩u M : ℕ[σ] @ ^(so_Some s) }} by (eapply glu_rel_exp_conv_unsorted; mauto 3).
+  assert {{ ⟪ pred_P ⟫ Δ with anns' ⊩u ℕ : Sort@s @ ^so_None }} by mauto 3.
   eapply glu_rel_sub_extend; mauto 3.
 Qed.
 
@@ -197,13 +197,13 @@ Qed.
 Lemma glu_rel_exp_natrec_zero_helper_sorted {P} (pred_P : PredicativeSig P) : forall {sn s anns Γ SbΓ A MZ MS Δ M σ ρ am typ_rel exp_rel} {r : Ru_nat P sn},
     {{ EG Γ ∈ glu_ctx_env pred_P anns ↘ SbΓ }} ->
     {{ Γ, ℕ ⊢ A : Sort@s }} ->
-    {{ ⟪ pred_P ⟫ Γ with anns ⊩u A[Id,,zero] @ ^(Some s) }} ->
-    {{ ⟪ pred_P ⟫ Γ with anns ⊩u MZ : A[Id,,zero] @ ^(Some s) }} ->
+    {{ ⟪ pred_P ⟫ Γ with anns ⊩u A[Id,,zero] @ ^(so_Some s) }} ->
+    {{ ⟪ pred_P ⟫ Γ with anns ⊩u MZ : A[Id,,zero] @ ^(so_Some s) }} ->
     {{ Γ, ℕ, A ⊢ MS : A[Wk∘Wk,,succ #1] }} ->
     {{ Δ ⊢ M ≈ zero : ℕ }} ->
     {{ Δ ⊢s σ ® ρ ∈ SbΓ }} ->
     {{ ⟦ A ⟧ ρ ↦ zero ↘ am }} ->
-    {{ DG am ∈ glu_typ_elem pred_P (Some s) ↘ typ_rel ↘ exp_rel }} ->
+    {{ DG am ∈ glu_typ_elem pred_P (so_Some s) ↘ typ_rel ↘ exp_rel }} ->
     exists r,
       {{ rec zero ⟦return A | zero -> MZ | succ -> MS end⟧ ρ ↘ r }} /\
         {{ Δ ⊢ rec M return A[q σ] | zero -> MZ[σ] | succ -> MS[q (q σ)] end : A[σ,,M] ® r ∈ exp_rel }}.
@@ -213,10 +213,10 @@ Proof.
   assert {{ ⟪ pred_P ⟫ Γ with anns ⊩ MZ : A[Id,,zero] @ s }} by mauto 2.
   assert {{ Γ ⊢ MZ : A[Id,,zero] }} by mauto 3.
   inversion HMZ as [SbΓ' []].
-  assert {{ ⟪ pred_P ⟫ Γ with anns ⊩u ℕ : Sort@sn @ ^None }} as [SbΓ'' []] by mauto 3.
+  assert {{ ⟪ pred_P ⟫ Γ with anns ⊩u ℕ : Sort@sn @ ^so_None }} as [SbΓ'' []] by mauto 3.
   handle_functional_glu_ctx_env P.
-  pose (SbΓℕ := cons_glu_sub_pred pred_P (Some sn) Γ {{{ ℕ }}} SbΓ'').
-  assert {{ EG Γ, ℕ ∈ glu_ctx_env pred_P ((Some sn)::anns) ↘ SbΓℕ }} by (econstructor; mauto 4; try reflexivity).
+  pose (SbΓℕ := cons_glu_sub_pred pred_P (so_Some sn) Γ {{{ ℕ }}} SbΓ'').
+  assert {{ EG Γ, ℕ ∈ glu_ctx_env pred_P ((so_Some sn)::anns) ↘ SbΓℕ }} by (econstructor; mauto 4; try reflexivity).
   handle_functional_glu_ctx_env P.
   invert_glu_rel_exp_unsorted H1.
   assert (forall (Δ : list (exp P)%type) (σ : sub P) (ρ : list (domain P)), SbΓ'' Δ σ ρ -> glu_rel_typ_with_sub pred_P sn Δ {{{ ℕ }}} σ ρ) by mauto 3.
@@ -279,13 +279,13 @@ Qed.
 Lemma glu_rel_exp_natrec_zero_helper_unsorted {P} (pred_P : PredicativeSig P) : forall {sn anns Γ SbΓ A MZ MS Δ M σ ρ am typ_rel exp_rel} {r : Ru_nat P sn},
     {{ EG Γ ∈ glu_ctx_env pred_P anns ↘ SbΓ }} ->
     {{ Γ, ℕ ⊢ A }} ->
-    {{ ⟪ pred_P ⟫ Γ with anns ⊩u A[Id,,zero] @ ^None }} ->
-    {{ ⟪ pred_P ⟫ Γ with anns ⊩u MZ : A[Id,,zero] @ ^None }} ->
+    {{ ⟪ pred_P ⟫ Γ with anns ⊩u A[Id,,zero] @ ^so_None }} ->
+    {{ ⟪ pred_P ⟫ Γ with anns ⊩u MZ : A[Id,,zero] @ ^so_None }} ->
     {{ Γ, ℕ, A ⊢ MS : A[Wk∘Wk,,succ #1] }} ->
     {{ Δ ⊢ M ≈ zero : ℕ }} ->
     {{ Δ ⊢s σ ® ρ ∈ SbΓ }} ->
     {{ ⟦ A ⟧ ρ ↦ zero ↘ am }} ->
-    {{ DG am ∈ glu_typ_elem pred_P None ↘ typ_rel ↘ exp_rel }} ->
+    {{ DG am ∈ glu_typ_elem pred_P so_None ↘ typ_rel ↘ exp_rel }} ->
     exists r,
       {{ rec zero ⟦return A | zero -> MZ | succ -> MS end⟧ ρ ↘ r }} /\
         {{ Δ ⊢ rec M return A[q σ] | zero -> MZ[σ] | succ -> MS[q (q σ)] end : A[σ,,M] ® r ∈ exp_rel }}.
@@ -293,10 +293,10 @@ Proof.
   intros * ? ? ? HMZ **.
   assert {{ Γ ⊢ MZ : A[Id,,zero] }} by mauto 3.
   inversion HMZ as [SbΓ' []].
-  assert {{ ⟪ pred_P ⟫ Γ with anns ⊩u ℕ : Sort@sn @ ^None }} as [SbΓ'' []] by mauto 3.
+  assert {{ ⟪ pred_P ⟫ Γ with anns ⊩u ℕ : Sort@sn @ ^so_None }} as [SbΓ'' []] by mauto 3.
   handle_functional_glu_ctx_env P.
-  pose (SbΓℕ := cons_glu_sub_pred pred_P (Some sn) Γ {{{ ℕ }}} SbΓ'').
-  assert {{ EG Γ, ℕ ∈ glu_ctx_env pred_P ((Some sn)::anns) ↘ SbΓℕ }} by (econstructor; mauto 4; try reflexivity).
+  pose (SbΓℕ := cons_glu_sub_pred pred_P (so_Some sn) Γ {{{ ℕ }}} SbΓ'').
+  assert {{ EG Γ, ℕ ∈ glu_ctx_env pred_P ((so_Some sn)::anns) ↘ SbΓℕ }} by (econstructor; mauto 4; try reflexivity).
   handle_functional_glu_ctx_env P.
   invert_glu_rel_exp_unsorted H1.
   assert (forall (Δ : list (exp P)%type) (σ : sub P) (ρ : list (domain P)), SbΓ'' Δ σ ρ -> glu_rel_typ_with_sub pred_P sn Δ {{{ ℕ }}} σ ρ) by mauto 3.
@@ -369,7 +369,7 @@ Lemma cons_glu_sub_pred_nat_helper {P} (pred_P : PredicativeSig P) : forall {ann
     {{ EG Γ ∈ glu_ctx_env pred_P anns ↘ SbΓ }} ->
     {{ Δ ⊢s σ ® ρ ∈ SbΓ }} ->
     glu_nat r Δ M m ->
-    {{ Δ ⊢s σ,,M ® ρ ↦ m ∈ cons_glu_sub_pred pred_P (Some s) Γ {{{ ℕ }}} SbΓ }}.
+    {{ Δ ⊢s σ,,M ® ρ ↦ m ∈ cons_glu_sub_pred pred_P (so_Some s) Γ {{{ ℕ }}} SbΓ }}.
 Proof.
   intros * ? HM ?.
   assert (st_subtyp s s) as Hst by mauto 2.  
@@ -384,43 +384,43 @@ Hint Resolve cons_glu_sub_pred_nat_helper : mcpts.
 
 Lemma glu_rel_exp_natrec_succ_helper_sorted {P} (pred_P : PredicativeSig P) : forall {s anns Γ SbΓ A MZ MS Δ M M' m' σ ρ am typ_rel exp_rel sn} {r : Ru_nat P sn},
     {{ EG Γ ∈ glu_ctx_env pred_P anns ↘ SbΓ }} ->
-    {{ ⟪ pred_P ⟫ Γ, ℕ with (Some sn)::anns ⊩u A @ ^(Some s) }} ->
+    {{ ⟪ pred_P ⟫ Γ, ℕ with (so_Some sn)::anns ⊩u A @ ^(so_Some s) }} ->
     {{ Γ ⊢ MZ : A[Id,,zero] }} ->
-    {{ ⟪ pred_P ⟫ Γ, ℕ, A with (Some s)::(Some sn)::anns ⊩u A[Wk∘Wk,,succ #1] @ ^(Some s) }} ->
-    {{ ⟪ pred_P ⟫ Γ, ℕ, A with (Some s)::(Some sn)::anns ⊩u MS : A[Wk∘Wk,,succ #1] @ ^(Some s) }} ->
+    {{ ⟪ pred_P ⟫ Γ, ℕ, A with (so_Some s)::(so_Some sn)::anns ⊩u A[Wk∘Wk,,succ #1] @ ^(so_Some s) }} ->
+    {{ ⟪ pred_P ⟫ Γ, ℕ, A with (so_Some s)::(so_Some sn)::anns ⊩u MS : A[Wk∘Wk,,succ #1] @ ^(so_Some s) }} ->
     {{ Δ ⊢ M ≈ succ M' : ℕ }} ->
     glu_nat r Δ M' m' ->
     (forall σ ρ am typ_rel exp_rel,
         {{ Δ ⊢s σ ® ρ ∈ SbΓ }} ->
         {{ ⟦ A ⟧ ρ ↦ m' ↘ am }} ->
-        {{ DG am ∈ glu_typ_elem pred_P (Some s) ↘ typ_rel ↘ exp_rel }} ->
+        {{ DG am ∈ glu_typ_elem pred_P (so_Some s) ↘ typ_rel ↘ exp_rel }} ->
         exists e,
           {{ rec m' ⟦return A | zero -> MZ | succ -> MS end⟧ ρ ↘ e }} /\
             {{ Δ ⊢ rec M' return A[q σ] | zero -> MZ[σ] | succ -> MS[q (q σ)] end : A[σ,,M'] ® e ∈ exp_rel }}) ->
     {{ Δ ⊢s σ ® ρ ∈ SbΓ }} ->
     {{ ⟦ A ⟧ ρ ↦ succ m' ↘ am }} ->
-    {{ DG am ∈ glu_typ_elem pred_P (Some s) ↘ typ_rel ↘ exp_rel }} ->
+    {{ DG am ∈ glu_typ_elem pred_P (so_Some s) ↘ typ_rel ↘ exp_rel }} ->
     exists e,
       {{ rec succ m' ⟦return A | zero -> MZ | succ -> MS end⟧ ρ ↘ e }} /\
         {{ Δ ⊢ rec M return A[q σ] | zero -> MZ[σ] | succ -> MS[q (q σ)] end : A[σ,,M] ® e ∈ exp_rel }}.
 Proof.
   intros * ? HA ? ? HMS **.
   assert {{ ⟪ pred_P ⟫ ⊩ Γ with anns }} by (eexists; eassumption).
-  assert {{ ⟪ pred_P ⟫ Γ with anns ⊩u ℕ : Sort@sn @ ^None }} as Hℕ by mauto 3.
-  pose (SbΓℕ := cons_glu_sub_pred pred_P (Some sn) Γ {{{ ℕ }}} SbΓ).
-  assert {{ EG Γ, ℕ  ∈ glu_ctx_env pred_P ((Some sn)::anns) ↘ SbΓℕ }} by (invert_glu_rel_exp_unsorted Hℕ; econstructor; mauto 4; try reflexivity).
+  assert {{ ⟪ pred_P ⟫ Γ with anns ⊩u ℕ : Sort@sn @ ^so_None }} as Hℕ by mauto 3.
+  pose (SbΓℕ := cons_glu_sub_pred pred_P (so_Some sn) Γ {{{ ℕ }}} SbΓ).
+  assert {{ EG Γ, ℕ  ∈ glu_ctx_env pred_P ((so_Some sn)::anns) ↘ SbΓℕ }} by (invert_glu_rel_exp_unsorted Hℕ; econstructor; mauto 4; try reflexivity).
 
 
   assert {{ Γ, ℕ ⊢ A : Sort@s }} by mauto 3.
   invert_glu_rel_typ_unsorted HA.
-  pose (SbΓℕA := cons_glu_sub_pred pred_P (Some s) {{{ Γ, ℕ }}} A SbΓℕ).
-  assert {{ EG Γ, ℕ, A ∈ glu_ctx_env pred_P ((Some s)::(Some sn)::anns) ↘ SbΓℕA }} by (econstructor; mauto 3; reflexivity).
+  pose (SbΓℕA := cons_glu_sub_pred pred_P (so_Some s) {{{ Γ, ℕ }}} A SbΓℕ).
+  assert {{ EG Γ, ℕ, A ∈ glu_ctx_env pred_P ((so_Some s)::(so_Some sn)::anns) ↘ SbΓℕA }} by (econstructor; mauto 3; reflexivity).
 
   assert {{ Γ, ℕ, A ⊢ MS : A[Wk∘Wk,,succ #1] }} by mauto 2.
   invert_glu_rel_exp_unsorted HMS.
   handle_functional_glu_ctx_env P.
   assert {{ Δ ⊢s σ,,M' ® ρ ↦ m' ∈ SbΓℕ }} by (unfold SbΓℕ; mauto 3).
-  assert (glu_rel_typ_with_sub_unsorted pred_P (Some s) Δ A {{{ σ,,M' }}} d{{{ ρ ↦ m' }}}) by mauto 3; subst.
+  assert (glu_rel_typ_with_sub_unsorted pred_P (so_Some s) Δ A {{{ σ,,M' }}} d{{{ ρ ↦ m' }}}) by mauto 3; subst.
   inversion H14; subst.
   match goal with
   | _: {{ ⟦ A ⟧ ^d{{{ ρ ↦ m' }}} ↘ ^?m }}, _: {{ DG ^?m ∈ glu_sort_elem pred_P ?s ↘ ?P ↘ ?El }} |- _ =>
@@ -565,43 +565,43 @@ Qed.
 
 Lemma glu_rel_exp_natrec_succ_helper_unsorted {P} (pred_P : PredicativeSig P) : forall {anns Γ SbΓ A MZ MS Δ M M' m' σ ρ am typ_rel exp_rel sn} {r : Ru_nat P sn},
     {{ EG Γ ∈ glu_ctx_env pred_P anns ↘ SbΓ }} ->
-    {{ ⟪ pred_P ⟫ Γ, ℕ with (Some sn)::anns ⊩u A @ ^None }} ->
+    {{ ⟪ pred_P ⟫ Γ, ℕ with (so_Some sn)::anns ⊩u A @ ^so_None }} ->
     {{ Γ ⊢ MZ : A[Id,,zero] }} ->
-    {{ ⟪ pred_P ⟫ Γ, ℕ, A with None::(Some sn)::anns ⊩u A[Wk∘Wk,,succ #1] @ ^None }} ->
-    {{ ⟪ pred_P ⟫ Γ, ℕ, A with None::(Some sn)::anns ⊩u MS : A[Wk∘Wk,,succ #1] @ ^None }} ->
+    {{ ⟪ pred_P ⟫ Γ, ℕ, A with so_None::(so_Some sn)::anns ⊩u A[Wk∘Wk,,succ #1] @ ^so_None }} ->
+    {{ ⟪ pred_P ⟫ Γ, ℕ, A with so_None::(so_Some sn)::anns ⊩u MS : A[Wk∘Wk,,succ #1] @ ^so_None }} ->
     {{ Δ ⊢ M ≈ succ M' : ℕ }} ->
     glu_nat r Δ M' m' ->
     (forall σ ρ am typ_rel exp_rel,
         {{ Δ ⊢s σ ® ρ ∈ SbΓ }} ->
         {{ ⟦ A ⟧ ρ ↦ m' ↘ am }} ->
-        {{ DG am ∈ glu_typ_elem pred_P None ↘ typ_rel ↘ exp_rel }} ->
+        {{ DG am ∈ glu_typ_elem pred_P so_None ↘ typ_rel ↘ exp_rel }} ->
         exists e,
           {{ rec m' ⟦return A | zero -> MZ | succ -> MS end⟧ ρ ↘ e }} /\
             {{ Δ ⊢ rec M' return A[q σ] | zero -> MZ[σ] | succ -> MS[q (q σ)] end : A[σ,,M'] ® e ∈ exp_rel }}) ->
     {{ Δ ⊢s σ ® ρ ∈ SbΓ }} ->
     {{ ⟦ A ⟧ ρ ↦ succ m' ↘ am }} ->
-    {{ DG am ∈ glu_typ_elem pred_P None ↘ typ_rel ↘ exp_rel }} ->
+    {{ DG am ∈ glu_typ_elem pred_P so_None ↘ typ_rel ↘ exp_rel }} ->
     exists e,
       {{ rec succ m' ⟦return A | zero -> MZ | succ -> MS end⟧ ρ ↘ e }} /\
         {{ Δ ⊢ rec M return A[q σ] | zero -> MZ[σ] | succ -> MS[q (q σ)] end : A[σ,,M] ® e ∈ exp_rel }}.
 Proof.
   intros * ? HA ? ? HMS **.
   assert {{ ⟪ pred_P ⟫ ⊩ Γ with anns }} by (eexists; eassumption).
-  assert {{ ⟪ pred_P ⟫ Γ with anns ⊩u ℕ : Sort@sn @ ^None }} as Hℕ by mauto 3.
-  pose (SbΓℕ := cons_glu_sub_pred pred_P (Some sn) Γ {{{ ℕ }}} SbΓ).
-  assert {{ EG Γ, ℕ  ∈ glu_ctx_env pred_P ((Some sn)::anns) ↘ SbΓℕ }} by (invert_glu_rel_exp_unsorted Hℕ; econstructor; mauto 4; try reflexivity).
+  assert {{ ⟪ pred_P ⟫ Γ with anns ⊩u ℕ : Sort@sn @ ^so_None }} as Hℕ by mauto 3.
+  pose (SbΓℕ := cons_glu_sub_pred pred_P (so_Some sn) Γ {{{ ℕ }}} SbΓ).
+  assert {{ EG Γ, ℕ  ∈ glu_ctx_env pred_P ((so_Some sn)::anns) ↘ SbΓℕ }} by (invert_glu_rel_exp_unsorted Hℕ; econstructor; mauto 4; try reflexivity).
 
 
   assert {{ Γ, ℕ ⊢ A }} by mauto 2.
   invert_glu_rel_typ_unsorted HA.
-  pose (SbΓℕA := cons_glu_sub_pred pred_P None {{{ Γ, ℕ }}} A SbΓℕ).
-  assert {{ EG Γ, ℕ, A ∈ glu_ctx_env pred_P (None::(Some sn)::anns) ↘ SbΓℕA }} by (econstructor; mauto 3; reflexivity).
+  pose (SbΓℕA := cons_glu_sub_pred pred_P so_None {{{ Γ, ℕ }}} A SbΓℕ).
+  assert {{ EG Γ, ℕ, A ∈ glu_ctx_env pred_P (so_None::(so_Some sn)::anns) ↘ SbΓℕA }} by (econstructor; mauto 3; reflexivity).
 
   assert {{ Γ, ℕ, A ⊢ MS : A[Wk∘Wk,,succ #1] }} by mauto 2.
   invert_glu_rel_exp_unsorted HMS.
   handle_functional_glu_ctx_env P.
   assert {{ Δ ⊢s σ,,M' ® ρ ↦ m' ∈ SbΓℕ }} by (unfold SbΓℕ; mauto 3).
-  assert (glu_rel_typ_with_sub_unsorted pred_P None Δ A {{{ σ,,M' }}} d{{{ ρ ↦ m' }}}) by mauto 3; subst.
+  assert (glu_rel_typ_with_sub_unsorted pred_P so_None Δ A {{{ σ,,M' }}} d{{{ ρ ↦ m' }}}) by mauto 3; subst.
   inversion H14; subst.
   functional_eval_rewrite_clear.
   match goal with
@@ -768,8 +768,8 @@ Proof.
     assert {{ Δ ⊢s σ : Γ }} by mauto 2;
     assert {{ ⊢ Δ, A[σ] }} by mauto 4;
     assert {{ Δ, A[σ] ⊢w Wk : Δ }} by mauto 2;
-    [assert (glu_rel_typ_with_sub_unsorted pred_P None Δ A σ ρ) by mauto 2 |
-      assert (glu_rel_typ_with_sub_unsorted pred_P (Some s) Δ A σ ρ) by mauto 2];
+    [assert (glu_rel_typ_with_sub_unsorted pred_P so_None Δ A σ ρ) by mauto 2 |
+      assert (glu_rel_typ_with_sub_unsorted pred_P (so_Some s) Δ A σ ρ) by mauto 2];
     inversion H6;
     simplify_evals.
   - eapply cons_glu_sub_pred_helper_unsorted; mauto 2.
@@ -791,15 +791,15 @@ Hint Resolve cons_glu_sub_pred_q_helper : mcpts.
 Lemma cons_glu_sub_pred_q_nat_helper {P} (pred_P : PredicativeSig P) : forall {anns Γ SbΓ Δ σ ρ s} {r : Ru_nat P s},
     {{ EG Γ ∈ glu_ctx_env pred_P anns ↘ SbΓ }} ->
     {{ Δ ⊢s σ ® ρ ∈ SbΓ }} ->
-    {{ Δ, ℕ ⊢s q σ ® ρ ↦ ⇑! ℕ (length Δ) ∈ cons_glu_sub_pred pred_P (Some s) Γ {{{ ℕ }}} SbΓ }}.
+    {{ Δ, ℕ ⊢s q σ ® ρ ↦ ⇑! ℕ (length Δ) ∈ cons_glu_sub_pred pred_P (so_Some s) Γ {{{ ℕ }}} SbΓ }}.
 Proof.
   intros.
   assert {{ ⟪ pred_P ⟫ ⊩ Γ with anns }} by (eexists; eassumption).
-  assert {{ ⟪ pred_P ⟫ Γ with anns ⊩u ℕ : Sort@s @ ^None }} as Hℕ by mauto 3.
+  assert {{ ⟪ pred_P ⟫ Γ with anns ⊩u ℕ : Sort@s @ ^so_None }} as Hℕ by mauto 3.
   assert {{ ⟦ ℕ ⟧ ρ ↘ ℕ }} by mauto 3.
-  assert {{ Δ, ℕ[σ] ⊢s q σ ® ρ ↦ ⇑! ℕ (length Δ) ∈ cons_glu_sub_pred pred_P (Some s) Γ {{{ ℕ }}} SbΓ }} by mauto 3.
+  assert {{ Δ, ℕ[σ] ⊢s q σ ® ρ ↦ ⇑! ℕ (length Δ) ∈ cons_glu_sub_pred pred_P (so_Some s) Γ {{{ ℕ }}} SbΓ }} by mauto 3.
   assert {{ Δ ⊢ ℕ[σ] ≈ ℕ : Sort@s }} by (econstructor; mauto 4).
-  assert {{ EG Γ, ℕ ∈ glu_ctx_env pred_P ((Some s)::anns) ↘ cons_glu_sub_pred pred_P (Some s) Γ {{{ ℕ }}} SbΓ }}.
+  assert {{ EG Γ, ℕ ∈ glu_ctx_env pred_P ((so_Some s)::anns) ↘ cons_glu_sub_pred pred_P (so_Some s) Γ {{{ ℕ }}} SbΓ }}.
   {
     invert_glu_rel_exp_unsorted Hℕ; destruct_conjs; econstructor; mauto 3.
     assert (forall (Δ : list (exp P)%type) (σ : sub P) (ρ : list (domain P)), SbΓ Δ σ ρ -> glu_rel_typ_with_sub pred_P s Δ {{{ ℕ }}} σ ρ) by mauto 3.
@@ -817,16 +817,16 @@ Qed.
 
 Lemma glu_rel_exp_natrec_neut_helper_sorted {P} (pred_P : PredicativeSig P) : forall {s anns Γ SbΓ A MZ MS Δ M a m σ ρ am typ_rel exp_rel sn} {r : Ru_nat P sn},
     {{ EG Γ ∈ glu_ctx_env pred_P anns ↘ SbΓ }} ->
-    {{ ⟪ pred_P ⟫ Γ, ℕ with (Some sn)::anns ⊩u A @ ^(Some s) }} ->
-    {{ ⟪ pred_P ⟫ Γ with anns ⊩u A[Id,,zero] @ ^(Some s) }} ->
-    {{ ⟪ pred_P ⟫ Γ with anns ⊩u MZ : A[Id,,zero] @ ^(Some s) }} ->
-    {{ ⟪ pred_P ⟫ Γ, ℕ, A with (Some s)::(Some sn)::anns ⊩u A[Wk∘Wk,,succ #1] @ ^(Some s) }} ->
-    {{ ⟪ pred_P ⟫ Γ, ℕ, A with (Some s)::(Some sn)::anns ⊩u MS : A[Wk∘Wk,,succ #1] @ ^(Some s) }} ->
+    {{ ⟪ pred_P ⟫ Γ, ℕ with (so_Some sn)::anns ⊩u A @ ^(so_Some s) }} ->
+    {{ ⟪ pred_P ⟫ Γ with anns ⊩u A[Id,,zero] @ ^(so_Some s) }} ->
+    {{ ⟪ pred_P ⟫ Γ with anns ⊩u MZ : A[Id,,zero] @ ^(so_Some s) }} ->
+    {{ ⟪ pred_P ⟫ Γ, ℕ, A with (so_Some s)::(so_Some sn)::anns ⊩u A[Wk∘Wk,,succ #1] @ ^(so_Some s) }} ->
+    {{ ⟪ pred_P ⟫ Γ, ℕ, A with (so_Some s)::(so_Some sn)::anns ⊩u MS : A[Wk∘Wk,,succ #1] @ ^(so_Some s) }} ->
     {{ Dom m ≈ m ∈ per_bot }} ->
     (forall Δ' τ V, {{ Δ' ⊢w τ : Δ }} -> {{ Rne m in length Δ' ↘ V }} -> {{ Δ' ⊢ M[τ] ≈ V : ℕ }}) ->
     {{ Δ ⊢s σ ® ρ ∈ SbΓ }} ->
     {{ ⟦ A ⟧ ρ ↦ ⇑ a m ↘ am }} ->
-    {{ DG am ∈ glu_typ_elem pred_P (Some s) ↘ typ_rel ↘ exp_rel }} ->
+    {{ DG am ∈ glu_typ_elem pred_P (so_Some s) ↘ typ_rel ↘ exp_rel }} ->
     exists e,
       {{ rec ⇑ a m ⟦return A | zero -> MZ | succ -> MS end⟧ ρ ↘ e }} /\
         {{ Δ ⊢ rec M return A[q σ] | zero -> MZ[σ] | succ -> MS[q (q σ)] end : A[σ,,M] ® e ∈ exp_rel }}.
@@ -835,15 +835,15 @@ Proof.
   assert {{ Γ ⊢ MZ : A[Id,,zero] }} by mauto 2.
   invert_glu_rel_exp_unsorted HMZ.
   assert {{ ⟪ pred_P ⟫ ⊩ Γ with anns }} by (eexists; eassumption).
-  assert {{ ⟪ pred_P ⟫ Γ with anns ⊩u ℕ : Sort@sn @ ^None }} as Hℕ by mauto 3.
-  pose (SbΓℕ := cons_glu_sub_pred pred_P (Some sn) Γ {{{ ℕ }}} SbΓ).
-  assert {{ EG Γ, ℕ ∈ glu_ctx_env pred_P ((Some sn)::anns) ↘ SbΓℕ }} by (invert_glu_rel_exp_unsorted Hℕ; econstructor; mauto 4; try reflexivity).
+  assert {{ ⟪ pred_P ⟫ Γ with anns ⊩u ℕ : Sort@sn @ ^so_None }} as Hℕ by mauto 3.
+  pose (SbΓℕ := cons_glu_sub_pred pred_P (so_Some sn) Γ {{{ ℕ }}} SbΓ).
+  assert {{ EG Γ, ℕ ∈ glu_ctx_env pred_P ((so_Some sn)::anns) ↘ SbΓℕ }} by (invert_glu_rel_exp_unsorted Hℕ; econstructor; mauto 4; try reflexivity).
   assert {{ Γ, ℕ ⊢ A : Sort@s }} by mauto 3.
   pose proof HA.
   invert_glu_rel_typ_unsorted HA.
-  assert (forall Δ σ ρ, SbΓℕ Δ σ ρ -> glu_rel_typ_with_sub_unsorted pred_P (Some s) Δ A σ ρ) by mauto 3.
-  pose (SbΓℕA := cons_glu_sub_pred pred_P (Some s) {{{ Γ, ℕ }}} A SbΓℕ).
-  assert {{ EG Γ, ℕ, A ∈ glu_ctx_env pred_P ((Some s)::(Some sn)::anns) ↘ SbΓℕA }} by (econstructor; mauto 3; reflexivity).
+  assert (forall Δ σ ρ, SbΓℕ Δ σ ρ -> glu_rel_typ_with_sub_unsorted pred_P (so_Some s) Δ A σ ρ) by mauto 3.
+  pose (SbΓℕA := cons_glu_sub_pred pred_P (so_Some s) {{{ Γ, ℕ }}} A SbΓℕ).
+  assert {{ EG Γ, ℕ, A ∈ glu_ctx_env pred_P ((so_Some s)::(so_Some sn)::anns) ↘ SbΓℕA }} by (econstructor; mauto 3; reflexivity).
 
   assert {{ Δ ⊢s σ,,M ® ρ ↦ ⇑ a m ∈ SbΓℕ }}.
   {
@@ -855,8 +855,8 @@ Proof.
   invert_glu_rel_exp_unsorted HMS.
   destruct_conjs.
   apply_functional_glu_ctx_env.
-  assert (glu_rel_typ_with_sub_unsorted pred_P (Some s) Δ A {{{ σ,,M }}} d{{{ ρ ↦ ⇑ a m }}}) by mauto 2.
-  assert (glu_rel_exp_with_sub_unsorted pred_P (Some s) Δ MZ {{{ A[Id,,zero] }}} σ ρ) by mauto 2.
+  assert (glu_rel_typ_with_sub_unsorted pred_P (so_Some s) Δ A {{{ σ,,M }}} d{{{ ρ ↦ ⇑ a m }}}) by mauto 2.
+  assert (glu_rel_exp_with_sub_unsorted pred_P (so_Some s) Δ MZ {{{ A[Id,,zero] }}} σ ρ) by mauto 2.
  
   
   destruct_glu_rel_typ_with_sub_unsorted.
@@ -902,7 +902,7 @@ Proof.
   assert {{ Δ, ℕ, A[q σ] ⊢ MS[q (q σ)] : A[Wk∘Wk,,succ #1][q (q σ)] }} by (eapply wf_exp_sub_typ; mauto 4).
   assert {{ Δ, ℕ, A[q σ] ⊢ MS[q (q σ)] : A[q σ][Wk∘Wk,,succ #1] }} by mauto 3.
   pose (R := {{{ rec M return A[q σ] | zero -> MZ[σ] | succ -> MS[q (q σ)] end }}}).
-  enough {{ Δ ⊢ R : A[σ,,M] ® rec m under ρ return A | zero -> mz | succ -> MS end ∈ glu_elem_bot_unsorted pred_P (Some s) am }} by (eapply realize_glu_elem_bot_unsorted; mauto 3).
+  enough {{ Δ ⊢ R : A[σ,,M] ® rec m under ρ return A | zero -> mz | succ -> MS end ∈ glu_elem_bot_unsorted pred_P (so_Some s) am }} by (eapply realize_glu_elem_bot_unsorted; mauto 3).
   econstructor; mauto 3.
   - assert {{ Δ ⊢ A[q σ][Id,,M] ≈ A[σ,,M] : Sort@s }} by mauto 2.
     eapply wf_conv'; mauto 3.
@@ -981,7 +981,7 @@ Proof.
     assert {{ Δ' ⊢s σ∘τ : Γ }} by mauto 3.
     assert {{ Δ' ⊢s σ∘τ ® ρ ∈ SbΓ }} by (eapply glu_ctx_env_sub_monotone; mauto 4).
     assert {{ Δ', ℕ ⊢s q (σ∘τ) ® ρ ↦ ⇑! ℕ (length Δ') ∈ SbΓℕ }} by (unfold SbΓℕ; mauto 3).
-    assert (forall (Δ : list (exp P)%type) (σ : sub P) (ρ : list (domain P)), SbΓℕ Δ σ ρ -> glu_rel_typ_with_sub_unsorted pred_P (Some s) Δ A σ ρ) by mauto 3.
+    assert (forall (Δ : list (exp P)%type) (σ : sub P) (ρ : list (domain P)), SbΓℕ Δ σ ρ -> glu_rel_typ_with_sub_unsorted pred_P (so_Some s) Δ A σ ρ) by mauto 3.
     destruct_glu_rel_typ_with_sub_unsorted.
     simplify_evals.
     dir_inversion_clear_by_head (@read_ne P).
@@ -992,7 +992,7 @@ Proof.
         rename a into aΔ'
     end.
     assert {{ Δ', ℕ, A[q (σ∘τ)] ⊢s q (q (σ∘τ)) ® (ρ ↦ ⇑! ℕ (length Δ')) ↦ ⇑! aΔ' (length {{{ Δ', ℕ }}}) ∈ SbΓℕA }} by (unfold SbΓℕA; mauto 3).
-    assert (glu_rel_typ_with_sub_unsorted pred_P (Some s) {{{ Δ', ℕ }}} A {{{ q (σ∘τ) }}}
+    assert (glu_rel_typ_with_sub_unsorted pred_P (so_Some s) {{{ Δ', ℕ }}} A {{{ q (σ∘τ) }}}
               d{{{ ρ ↦ ⇑! ℕ (length Δ') }}}) as Hglu_typ_unsorted by mauto 2.
     inversion Hglu_typ_unsorted; subst.
     destruct_glu_rel_exp_with_sub_unsorted.
@@ -1010,7 +1010,7 @@ Proof.
         rename MZ into MZ';
         rename M into M'
     end.
-    assert {{ Δ', ℕ ⊢ A[q (σ∘τ)] ® glu_typ_top_unsorted pred_P (Some s) aΔ' }} as Hglu_typ_top by (eapply realize_glu_typ_top_unsorted; mauto 3; econstructor; mauto 2).
+    assert {{ Δ', ℕ ⊢ A[q (σ∘τ)] ® glu_typ_top_unsorted pred_P (so_Some s) aΔ' }} as Hglu_typ_top by (eapply realize_glu_typ_top_unsorted; mauto 3; econstructor; mauto 2).
     inversion Hglu_typ_top; subst.
     assert {{ Δ ⊢ MZ[σ] : A[Id,,zero][σ] ® mz ∈ glu_elem_top pred_P s az }} as [] by (eapply realize_glu_elem_top; eassumption).
     assert {{ Δ', ℕ, A[q (σ∘τ)] ⊢ MS[q (q (σ∘τ))] : A[Wk∘Wk,,succ #1][q (q (σ∘τ))] ® ms ∈ glu_elem_top pred_P s asucc }} as []
@@ -1093,16 +1093,16 @@ Qed.
 
 Lemma glu_rel_exp_natrec_neut_helper_unsorted {P} (pred_P : PredicativeSig P) : forall {anns Γ SbΓ A MZ MS Δ M a m σ ρ am typ_rel exp_rel sn} {r : Ru_nat P sn},
     {{ EG Γ ∈ glu_ctx_env pred_P anns ↘ SbΓ }} ->
-    {{ ⟪ pred_P ⟫ Γ, ℕ with (Some sn)::anns ⊩u A @ ^None }} ->
-    {{ ⟪ pred_P ⟫ Γ with anns ⊩u A[Id,,zero] @ ^None }} ->
-    {{ ⟪ pred_P ⟫ Γ with anns ⊩u MZ : A[Id,,zero] @ ^None }} ->
-    {{ ⟪ pred_P ⟫ Γ, ℕ, A with None::(Some sn)::anns ⊩u A[Wk∘Wk,,succ #1] @ ^None }} ->
-    {{ ⟪ pred_P ⟫ Γ, ℕ, A with None::(Some sn)::anns ⊩u MS : A[Wk∘Wk,,succ #1] @ ^None }} ->
+    {{ ⟪ pred_P ⟫ Γ, ℕ with (so_Some sn)::anns ⊩u A @ ^so_None }} ->
+    {{ ⟪ pred_P ⟫ Γ with anns ⊩u A[Id,,zero] @ ^so_None }} ->
+    {{ ⟪ pred_P ⟫ Γ with anns ⊩u MZ : A[Id,,zero] @ ^so_None }} ->
+    {{ ⟪ pred_P ⟫ Γ, ℕ, A with so_None::(so_Some sn)::anns ⊩u A[Wk∘Wk,,succ #1] @ ^so_None }} ->
+    {{ ⟪ pred_P ⟫ Γ, ℕ, A with so_None::(so_Some sn)::anns ⊩u MS : A[Wk∘Wk,,succ #1] @ ^so_None }} ->
     {{ Dom m ≈ m ∈ per_bot }} ->
     (forall Δ' τ V, {{ Δ' ⊢w τ : Δ }} -> {{ Rne m in length Δ' ↘ V }} -> {{ Δ' ⊢ M[τ] ≈ V : ℕ }}) ->
     {{ Δ ⊢s σ ® ρ ∈ SbΓ }} ->
     {{ ⟦ A ⟧ ρ ↦ ⇑ a m ↘ am }} ->
-    {{ DG am ∈ glu_typ_elem pred_P (None) ↘ typ_rel ↘ exp_rel }} ->
+    {{ DG am ∈ glu_typ_elem pred_P (so_None) ↘ typ_rel ↘ exp_rel }} ->
     exists e,
       {{ rec ⇑ a m ⟦return A | zero -> MZ | succ -> MS end⟧ ρ ↘ e }} /\
         {{ Δ ⊢ rec M return A[q σ] | zero -> MZ[σ] | succ -> MS[q (q σ)] end : A[σ,,M] ® e ∈ exp_rel }}.
@@ -1111,15 +1111,15 @@ Proof.
   assert {{ Γ ⊢ MZ : A[Id,,zero] }} by mauto 2.
   invert_glu_rel_exp_unsorted HMZ.
   assert {{ ⟪ pred_P ⟫ ⊩ Γ with anns }} by (eexists; eassumption).
-  assert {{ ⟪ pred_P ⟫ Γ with anns ⊩u ℕ : Sort@sn @ ^None }} as Hℕ by mauto 3.
-  pose (SbΓℕ := cons_glu_sub_pred pred_P (Some sn) Γ {{{ ℕ }}} SbΓ).
-  assert {{ EG Γ, ℕ ∈ glu_ctx_env pred_P ((Some sn)::anns) ↘ SbΓℕ }} by (invert_glu_rel_exp_unsorted Hℕ; econstructor; mauto 4; try reflexivity).
+  assert {{ ⟪ pred_P ⟫ Γ with anns ⊩u ℕ : Sort@sn @ ^so_None }} as Hℕ by mauto 3.
+  pose (SbΓℕ := cons_glu_sub_pred pred_P (so_Some sn) Γ {{{ ℕ }}} SbΓ).
+  assert {{ EG Γ, ℕ ∈ glu_ctx_env pred_P ((so_Some sn)::anns) ↘ SbΓℕ }} by (invert_glu_rel_exp_unsorted Hℕ; econstructor; mauto 4; try reflexivity).
   assert {{ Γ, ℕ ⊢ A }} by mauto 3.
   pose proof HA.
   invert_glu_rel_typ_unsorted HA.
-  assert (forall Δ σ ρ, SbΓℕ Δ σ ρ -> glu_rel_typ_with_sub_unsorted pred_P None Δ A σ ρ) by mauto 3.
-  pose (SbΓℕA := cons_glu_sub_pred pred_P None {{{ Γ, ℕ }}} A SbΓℕ).
-  assert {{ EG Γ, ℕ, A ∈ glu_ctx_env pred_P (None::(Some sn)::anns) ↘ SbΓℕA }} by (econstructor; mauto 3; reflexivity).
+  assert (forall Δ σ ρ, SbΓℕ Δ σ ρ -> glu_rel_typ_with_sub_unsorted pred_P so_None Δ A σ ρ) by mauto 3.
+  pose (SbΓℕA := cons_glu_sub_pred pred_P so_None {{{ Γ, ℕ }}} A SbΓℕ).
+  assert {{ EG Γ, ℕ, A ∈ glu_ctx_env pred_P (so_None::(so_Some sn)::anns) ↘ SbΓℕA }} by (econstructor; mauto 3; reflexivity).
 
   assert {{ Δ ⊢s σ,,M ® ρ ↦ ⇑ a m ∈ SbΓℕ }}.
   {
@@ -1131,8 +1131,8 @@ Proof.
   invert_glu_rel_exp_unsorted HMS.
   destruct_conjs.
   apply_functional_glu_ctx_env.
-  assert (glu_rel_typ_with_sub_unsorted pred_P None Δ A {{{ σ,,M }}} d{{{ ρ ↦ ⇑ a m }}}) by mauto 2.
-  assert (glu_rel_exp_with_sub_unsorted pred_P None Δ MZ {{{ A[Id,,zero] }}} σ ρ) by mauto 2.
+  assert (glu_rel_typ_with_sub_unsorted pred_P so_None Δ A {{{ σ,,M }}} d{{{ ρ ↦ ⇑ a m }}}) by mauto 2.
+  assert (glu_rel_exp_with_sub_unsorted pred_P so_None Δ MZ {{{ A[Id,,zero] }}} σ ρ) by mauto 2.
  
   
   destruct_glu_rel_typ_with_sub_unsorted.
@@ -1177,12 +1177,12 @@ Proof.
   assert {{ Δ, ℕ, A[q σ] ⊢ MS[q (q σ)] : A[Wk∘Wk,,succ #1][q (q σ)] }} by (eapply wf_exp_sub_typ; mauto 4).
   assert {{ Δ, ℕ, A[q σ] ⊢ MS[q (q σ)] : A[q σ][Wk∘Wk,,succ #1] }} by mauto 3.
   pose (R := {{{ rec M return A[q σ] | zero -> MZ[σ] | succ -> MS[q (q σ)] end }}}).
-  enough {{ Δ ⊢ R : A[σ,,M] ® rec m under ρ return A | zero -> mz | succ -> MS end ∈ glu_elem_bot_unsorted pred_P None d{{{ Sort@s }}} }} by (eapply realize_glu_elem_bot_unsorted; mauto 3).
+  enough {{ Δ ⊢ R : A[σ,,M] ® rec m under ρ return A | zero -> mz | succ -> MS end ∈ glu_elem_bot_unsorted pred_P so_None d{{{ Sort@s }}} }} by (eapply realize_glu_elem_bot_unsorted; mauto 3).
 
   econstructor; mauto 3.
   - assert {{ Δ ⊢ A[q σ][Id,,M] ≈ A[σ,,M] }} by mauto 2.
     eapply wf_conv_typ; mauto 4.
-  - assert {{ Δ ⊢ MZ[σ] : A[Id,,zero][σ] ® mz ∈ glu_elem_top_unsorted pred_P None d{{{ Sort@s0 }}} }} as Hglu_top_unsorted by (eapply realize_glu_elem_top_unsorted; eassumption).
+  - assert {{ Δ ⊢ MZ[σ] : A[Id,,zero][σ] ® mz ∈ glu_elem_top_unsorted pred_P so_None d{{{ Sort@s0 }}} }} as Hglu_top_unsorted by (eapply realize_glu_elem_top_unsorted; eassumption).
     inversion Hglu_top_unsorted; subst.
     (* inversion H22; subst. *)
     (* inversion H6; subst. *)
@@ -1262,7 +1262,7 @@ Proof.
     assert {{ Δ' ⊢s σ∘τ : Γ }} by mauto 3.
     assert {{ Δ' ⊢s σ∘τ ® ρ ∈ SbΓ }} by (eapply glu_ctx_env_sub_monotone; mauto 4).
     assert {{ Δ', ℕ ⊢s q (σ∘τ) ® ρ ↦ ⇑! ℕ (length Δ') ∈ SbΓℕ }} by (unfold SbΓℕ; mauto 3).
-    assert (forall Δ σ ρ, SbΓℕ Δ σ ρ -> glu_rel_typ_with_sub_unsorted pred_P None Δ A σ ρ) by mauto 3.
+    assert (forall Δ σ ρ, SbΓℕ Δ σ ρ -> glu_rel_typ_with_sub_unsorted pred_P so_None Δ A σ ρ) by mauto 3.
     destruct_glu_rel_typ_with_sub_unsorted.
     simplify_evals.
     dir_inversion_clear_by_head (@read_ne P).
@@ -1273,9 +1273,9 @@ Proof.
         rename a into aΔ'
     end.
     assert {{ Δ', ℕ, A[q (σ∘τ)] ⊢s q (q (σ∘τ)) ® (ρ ↦ ⇑! ℕ (length Δ')) ↦ ⇑! aΔ' (length {{{ Δ', ℕ }}}) ∈ SbΓℕA }} by (unfold SbΓℕA; mauto 3).
-    assert (glu_rel_typ_with_sub_unsorted pred_P None {{{ Δ', ℕ }}} A {{{ q (σ∘τ) }}}
+    assert (glu_rel_typ_with_sub_unsorted pred_P so_None {{{ Δ', ℕ }}} A {{{ q (σ∘τ) }}}
               d{{{ ρ ↦ ⇑! ℕ (length Δ') }}}) as Hglu_typ_unsorted by mauto 2.
-    assert (glu_rel_exp_with_sub_unsorted pred_P None Δ MZ {{{ A[Id,,zero] }}} σ ρ) by mauto 2.
+    assert (glu_rel_exp_with_sub_unsorted pred_P so_None Δ MZ {{{ A[Id,,zero] }}} σ ρ) by mauto 2.
     inversion Hglu_typ_unsorted; subst.
     (* inversion H62; subst. *)
     destruct_glu_rel_exp_with_sub_unsorted.
@@ -1298,13 +1298,13 @@ Proof.
     end.
     inversion H61; subst.
     rename M1 into MZ.
-    assert {{ Δ', ℕ ⊢ A[q (σ∘τ)] ® glu_typ_top_unsorted pred_P None d{{{ Sort@s1 }}} }} as Hglu_typ_top by (eapply realize_glu_typ_top_unsorted; mauto 3; econstructor; mauto 2).
+    assert {{ Δ', ℕ ⊢ A[q (σ∘τ)] ® glu_typ_top_unsorted pred_P so_None d{{{ Sort@s1 }}} }} as Hglu_typ_top by (eapply realize_glu_typ_top_unsorted; mauto 3; econstructor; mauto 2).
     inversion Hglu_typ_top; subst.
     inversion H62; subst; clear H62.
-    assert {{ Δ ⊢ MZ[σ] : A[Id,,zero][σ] ® mz ∈ glu_elem_top_unsorted pred_P None d{{{ Sort@s0 }}} }} as Hglu_typ_top' by (eapply realize_glu_elem_top_unsorted; eassumption).
+    assert {{ Δ ⊢ MZ[σ] : A[Id,,zero][σ] ® mz ∈ glu_elem_top_unsorted pred_P so_None d{{{ Sort@s0 }}} }} as Hglu_typ_top' by (eapply realize_glu_elem_top_unsorted; eassumption).
     inversion Hglu_typ_top'; subst.
     
-    assert {{ Δ', ℕ, A[q (σ∘τ)] ⊢ MS[q (q (σ∘τ))] : A[Wk∘Wk,,succ #1][q (q (σ∘τ))] ® ms ∈ glu_elem_top_unsorted pred_P None d{{{ Sort@s2 }}} }} as Hglu_elem_top by (eapply realize_glu_elem_top_unsorted; mauto 3).
+    assert {{ Δ', ℕ, A[q (σ∘τ)] ⊢ MS[q (q (σ∘τ))] : A[Wk∘Wk,,succ #1][q (q (σ∘τ))] ® ms ∈ glu_elem_top_unsorted pred_P so_None d{{{ Sort@s2 }}} }} as Hglu_elem_top by (eapply realize_glu_elem_top_unsorted; mauto 3).
     inversion Hglu_elem_top; subst.
     assert {{ Δ ⊢s σ,,M : Γ, ℕ }} by mauto 4.
     assert {{ Δ' ⊢s σ∘τ,,M[τ] : Γ, ℕ }} by mauto 4.
@@ -1386,9 +1386,9 @@ Qed.
 
 Lemma glu_rel_exp_natrec_helper {P} (pred_P : PredicativeSig P) : forall {sn so anns Γ SbΓ A MZ MS} {r : Ru_nat P sn},
     {{ EG Γ ∈ glu_ctx_env pred_P anns ↘ SbΓ }} ->
-    {{ ⟪ pred_P ⟫ Γ, ℕ with (Some sn)::anns ⊩u A @ so }} ->
+    {{ ⟪ pred_P ⟫ Γ, ℕ with (so_Some sn)::anns ⊩u A @ so }} ->
     {{ ⟪ pred_P ⟫ Γ with anns ⊩u MZ : A[Id,,zero] @ so }} ->
-    {{ ⟪ pred_P ⟫ Γ, ℕ, A with so::(Some sn)::anns ⊩u MS : A[Wk∘Wk,,succ #1] @ so }} ->
+    {{ ⟪ pred_P ⟫ Γ, ℕ, A with so::(so_Some sn)::anns ⊩u MS : A[Wk∘Wk,,succ #1] @ so }} ->
     forall {Δ M m},
       glu_nat r Δ M m ->
       forall {σ ρ am P El},
@@ -1401,33 +1401,33 @@ Lemma glu_rel_exp_natrec_helper {P} (pred_P : PredicativeSig P) : forall {sn so 
 Proof.
   intros * ? HA ? ?.
   assert {{ ⟪ pred_P ⟫ ⊩ Γ with anns }} by mauto 3.
-  assert {{ ⟪ pred_P ⟫ Γ with anns ⊩u ℕ : Sort@sn @ ^None }} as Hℕ by mauto 3.
+  assert {{ ⟪ pred_P ⟫ Γ with anns ⊩u ℕ : Sort@sn @ ^so_None }} as Hℕ by mauto 3.
   assert {{ ⟪ pred_P ⟫ Γ with anns ⊩u A[Id,,zero] @ so }}.
   {
     assert {{ Γ ⊢ ℕ : Sort@sn }} by mauto 2.
     assert {{ Γ ⊢ ℕ ≈ ℕ[Id] : Sort@sn }} by mauto 4.
     mauto.
   }
-  pose (SbΓℕ := cons_glu_sub_pred pred_P (Some sn) Γ {{{ ℕ }}} SbΓ).
-  assert {{ EG Γ, ℕ ∈ glu_ctx_env pred_P ((Some sn)::anns) ↘ SbΓℕ }} by (invert_glu_rel_exp_unsorted Hℕ; econstructor; mauto 4; try reflexivity).
+  pose (SbΓℕ := cons_glu_sub_pred pred_P (so_Some sn) Γ {{{ ℕ }}} SbΓ).
+  assert {{ EG Γ, ℕ ∈ glu_ctx_env pred_P ((so_Some sn)::anns) ↘ SbΓℕ }} by (invert_glu_rel_exp_unsorted Hℕ; econstructor; mauto 4; try reflexivity).
   pose proof HA.
   invert_glu_rel_typ_unsorted HA.
   assert (forall Δ σ ρ, SbΓℕ Δ σ ρ -> glu_rel_typ_with_sub_unsorted pred_P so Δ A σ ρ) by mauto 3.
-  assert {{ ⟪ pred_P ⟫ Γ, ℕ, A with so::(Some sn)::anns ⊩u A[Wk∘Wk,,succ #1] @ so }}.
+  assert {{ ⟪ pred_P ⟫ Γ, ℕ, A with so::(so_Some sn)::anns ⊩u A[Wk∘Wk,,succ #1] @ so }}.
   {
-    assert {{ ⟪ pred_P ⟫ ⊩ Γ, ℕ, A with so::(Some sn)::anns }} by mauto 3.
-    assert {{ ⟪ pred_P ⟫ Γ, ℕ with (Some sn)::anns ⊩s Wk : Γ with anns }} by mauto 4.
-    assert {{ ⟪ pred_P ⟫ Γ, ℕ, A with so::(Some sn)::anns ⊩s Wk : Γ, ℕ with (Some sn)::anns }} by mauto 3.
+    assert {{ ⟪ pred_P ⟫ ⊩ Γ, ℕ, A with so::(so_Some sn)::anns }} by mauto 3.
+    assert {{ ⟪ pred_P ⟫ Γ, ℕ with (so_Some sn)::anns ⊩s Wk : Γ with anns }} by mauto 4.
+    assert {{ ⟪ pred_P ⟫ Γ, ℕ, A with so::(so_Some sn)::anns ⊩s Wk : Γ, ℕ with (so_Some sn)::anns }} by mauto 3.
     assert {{ Γ, ℕ ⊢s Wk : Γ }} by mauto 3.
     assert {{ Γ, ℕ, A ⊢s Wk : Γ, ℕ }} by mauto 3.
     assert {{ Γ, ℕ, A ⊢ ℕ[Wk][Wk] ≈ ℕ : Sort@sn }} by mauto 3.
     assert {{ Γ, ℕ, A ⊢ ℕ[Wk][Wk] ⊆ ℕ }} by mauto 3.
-    assert {{ ⟪ pred_P ⟫ Γ, ℕ, A with so::(Some sn)::anns ⊩u  ℕ : Sort@sn @ ^None }} by mauto 3.
-    assert {{ #1 : ℕ[Wk][Wk] @ (Some sn) ∈ Γ, ℕ, A with so::(Some sn)::anns }} by mauto 2.
-    assert {{ ⟪ pred_P ⟫ Γ, ℕ, A with so::(Some sn)::anns ⊩ #1 : ℕ[Wk][Wk] @ ^ sn }} by mauto 4.
-    assert {{ ⟪ pred_P ⟫ Γ, ℕ, A with so::(Some sn)::anns ⊩ #1 : ℕ @ sn }} by mauto 4.
-    assert {{ ⟪ pred_P ⟫ Γ, ℕ, A with so::(Some sn)::anns  ⊩ succ #1 : ℕ @ sn }} by mauto 4.
-    assert {{ ⟪ pred_P ⟫ Γ, ℕ, A with so::(Some sn)::anns ⊩u succ #1 : ℕ @ ^ (Some sn) }} by mauto 3.
+    assert {{ ⟪ pred_P ⟫ Γ, ℕ, A with so::(so_Some sn)::anns ⊩u  ℕ : Sort@sn @ ^so_None }} by mauto 3.
+    assert {{ #1 : ℕ[Wk][Wk] @ (so_Some sn) ∈ Γ, ℕ, A with so::(so_Some sn)::anns }} by mauto 2.
+    assert {{ ⟪ pred_P ⟫ Γ, ℕ, A with so::(so_Some sn)::anns ⊩ #1 : ℕ[Wk][Wk] @ ^ sn }} by mauto 4.
+    assert {{ ⟪ pred_P ⟫ Γ, ℕ, A with so::(so_Some sn)::anns ⊩ #1 : ℕ @ sn }} by mauto 4.
+    assert {{ ⟪ pred_P ⟫ Γ, ℕ, A with so::(so_Some sn)::anns  ⊩ succ #1 : ℕ @ sn }} by mauto 4.
+    assert {{ ⟪ pred_P ⟫ Γ, ℕ, A with so::(so_Some sn)::anns ⊩u succ #1 : ℕ @ ^ (so_Some sn) }} by mauto 3.
     mauto 4.
   }
   destruct so; induction 1; intros; rename Γ0 into Δ.
@@ -1459,25 +1459,25 @@ Qed.
   
 
 Lemma glu_rel_exp_natrec_sorted {P} (pred_P : PredicativeSig P) : forall {sn s anns Γ A MZ MS M} {r : Ru_nat P sn},
-    {{ ⟪ pred_P ⟫ Γ, ℕ with (Some sn)::anns ⊩u A @ ^(Some s) }} ->
-    {{ ⟪ pred_P ⟫ Γ with anns ⊩u MZ : A[Id,,zero] @ ^(Some s) }} ->
-    {{ ⟪ pred_P ⟫ Γ, ℕ, A with (Some s)::(Some sn)::anns ⊩u MS : A[Wk∘Wk,,succ #1] @ ^(Some s) }} ->
+    {{ ⟪ pred_P ⟫ Γ, ℕ with (so_Some sn)::anns ⊩u A @ ^(so_Some s) }} ->
+    {{ ⟪ pred_P ⟫ Γ with anns ⊩u MZ : A[Id,,zero] @ ^(so_Some s) }} ->
+    {{ ⟪ pred_P ⟫ Γ, ℕ, A with (so_Some s)::(so_Some sn)::anns ⊩u MS : A[Wk∘Wk,,succ #1] @ ^(so_Some s) }} ->
     {{ ⟪ pred_P ⟫ Γ with anns ⊩ M : ℕ @ sn }} ->
-    {{ ⟪ pred_P ⟫ Γ with anns ⊩u rec M return A | zero -> MZ | succ -> MS end : A[Id,,M] @ ^(Some s) }}.
+    {{ ⟪ pred_P ⟫ Γ with anns ⊩u rec M return A | zero -> MZ | succ -> MS end : A[Id,,M] @ ^(so_Some s) }}.
 Proof.
   intros * r HA HMZ HMS HM.
   assert {{ Γ, ℕ ⊢ A : Sort@s }} by mauto 3.
   assert {{ ⟪ pred_P ⟫ ⊩ Γ with anns }} as [SbΓ] by mauto 3.
-  assert {{ ⟪ pred_P ⟫ Γ with anns ⊩u ℕ : Sort@sn @ ^None }} as Hℕ by mauto 4.
-  pose (SbΓℕ := cons_glu_sub_pred pred_P (Some sn) Γ {{{ ℕ }}} SbΓ).
-  assert {{ EG Γ, ℕ ∈ glu_ctx_env pred_P ((Some sn)::anns)↘ SbΓℕ }} by (invert_glu_rel_exp_unsorted Hℕ; econstructor; mauto 4; reflexivity).
-  pose (SbΓℕA := cons_glu_sub_pred pred_P (Some s) {{{ Γ, ℕ }}} {{{ A }}} SbΓℕ).
-  assert {{ EG Γ, ℕ, A ∈ glu_ctx_env pred_P ((Some s)::(Some sn)::anns) ↘ SbΓℕA }} by (invert_glu_rel_typ_unsorted HA; econstructor; mauto 4; try reflexivity).
+  assert {{ ⟪ pred_P ⟫ Γ with anns ⊩u ℕ : Sort@sn @ ^so_None }} as Hℕ by mauto 4.
+  pose (SbΓℕ := cons_glu_sub_pred pred_P (so_Some sn) Γ {{{ ℕ }}} SbΓ).
+  assert {{ EG Γ, ℕ ∈ glu_ctx_env pred_P ((so_Some sn)::anns)↘ SbΓℕ }} by (invert_glu_rel_exp_unsorted Hℕ; econstructor; mauto 4; reflexivity).
+  pose (SbΓℕA := cons_glu_sub_pred pred_P (so_Some s) {{{ Γ, ℕ }}} {{{ A }}} SbΓℕ).
+  assert {{ EG Γ, ℕ, A ∈ glu_ctx_env pred_P ((so_Some s)::(so_Some sn)::anns) ↘ SbΓℕA }} by (invert_glu_rel_typ_unsorted HA; econstructor; mauto 4; try reflexivity).
   pose proof HM.
   invert_glu_rel_exp HM.
   pose proof HA.
   invert_glu_rel_typ_unsorted HA.
-  assert (forall Δ σ ρ, SbΓℕ Δ σ ρ -> glu_rel_typ_with_sub_unsorted pred_P (Some s) Δ A σ ρ) by mauto 3.
+  assert (forall Δ σ ρ, SbΓℕ Δ σ ρ -> glu_rel_typ_with_sub_unsorted pred_P (so_Some s) Δ A σ ρ) by mauto 3.
   (* eapply glu_rel_exp_implies_glu_rel_exp_unsorted. *)
   eexists; split; [eassumption |].
   intros.
@@ -1488,7 +1488,7 @@ Proof.
   inversion_clear_by_head (@nat_glu_exp_pred P).
   assert (glu_nat r Δ {{{ M[σ] }}} m) by mauto 2.
   assert {{ Δ ⊢s σ,,M[σ] ® ρ ↦ m ∈ SbΓℕ }} by (unfold SbΓℕ; mauto 3).
-  assert (glu_rel_typ_with_sub_unsorted pred_P (Some s) Δ A {{{ σ,,M[σ] }}} d{{{ ρ ↦ m }}}) by mauto 2.
+  assert (glu_rel_typ_with_sub_unsorted pred_P (so_Some s) Δ A {{{ σ,,M[σ] }}} d{{{ ρ ↦ m }}}) by mauto 2.
   inversion H12; subst.
 
   assert (exists r, {{ rec m ⟦return A | zero -> MZ | succ -> MS end⟧ ρ ↘ r }} /\ exp_rel Δ {{{ A[σ,, M[σ]] }}} {{{ rec M[σ] return A[q σ] | zero -> MZ[σ] | succ -> MS[q (q σ)] end }}} r) as [? []] by (eapply glu_rel_exp_natrec_helper; revgoals; mauto 4; econstructor; mauto 2).
@@ -1502,25 +1502,25 @@ Proof.
 Qed.
 
 Lemma glu_rel_exp_natrec_unsorted {P} (pred_P : PredicativeSig P) : forall {sn anns Γ A MZ MS M} {r : Ru_nat P sn},
-    {{ ⟪ pred_P ⟫ Γ, ℕ with (Some sn)::anns ⊩u A @ ^None }} ->
-    {{ ⟪ pred_P ⟫ Γ with anns ⊩u MZ : A[Id,,zero] @ ^None }} ->
-    {{ ⟪ pred_P ⟫ Γ, ℕ, A with None::(Some sn)::anns ⊩u MS : A[Wk∘Wk,,succ #1] @ ^None }} ->
+    {{ ⟪ pred_P ⟫ Γ, ℕ with (so_Some sn)::anns ⊩u A @ ^so_None }} ->
+    {{ ⟪ pred_P ⟫ Γ with anns ⊩u MZ : A[Id,,zero] @ ^so_None }} ->
+    {{ ⟪ pred_P ⟫ Γ, ℕ, A with so_None::(so_Some sn)::anns ⊩u MS : A[Wk∘Wk,,succ #1] @ ^so_None }} ->
     {{ ⟪ pred_P ⟫ Γ with anns ⊩ M : ℕ @ sn }} ->
-    {{ ⟪ pred_P ⟫ Γ with anns ⊩u rec M return A | zero -> MZ | succ -> MS end : A[Id,,M] @ ^None }}.
+    {{ ⟪ pred_P ⟫ Γ with anns ⊩u rec M return A | zero -> MZ | succ -> MS end : A[Id,,M] @ ^so_None }}.
 Proof.
   intros * r HA HMZ HMS HM.
   assert {{ Γ, ℕ ⊢ A }} by mauto 3.
   assert {{ ⟪ pred_P ⟫ ⊩ Γ with anns }} as [SbΓ] by mauto 3.
-  assert {{ ⟪ pred_P ⟫ Γ with anns ⊩u ℕ : Sort@sn @ ^None }} as Hℕ by mauto 4.
-  pose (SbΓℕ := cons_glu_sub_pred pred_P (Some sn) Γ {{{ ℕ }}} SbΓ).
-  assert {{ EG Γ, ℕ ∈ glu_ctx_env pred_P ((Some sn)::anns)↘ SbΓℕ }} by (invert_glu_rel_exp_unsorted Hℕ; econstructor; mauto 4; reflexivity).
-  pose (SbΓℕA := cons_glu_sub_pred pred_P None {{{ Γ, ℕ }}} {{{ A }}} SbΓℕ).
-  assert {{ EG Γ, ℕ, A ∈ glu_ctx_env pred_P (None::(Some sn)::anns) ↘ SbΓℕA }} by (invert_glu_rel_typ_unsorted HA; econstructor; mauto 4; try reflexivity).
+  assert {{ ⟪ pred_P ⟫ Γ with anns ⊩u ℕ : Sort@sn @ ^so_None }} as Hℕ by mauto 4.
+  pose (SbΓℕ := cons_glu_sub_pred pred_P (so_Some sn) Γ {{{ ℕ }}} SbΓ).
+  assert {{ EG Γ, ℕ ∈ glu_ctx_env pred_P ((so_Some sn)::anns)↘ SbΓℕ }} by (invert_glu_rel_exp_unsorted Hℕ; econstructor; mauto 4; reflexivity).
+  pose (SbΓℕA := cons_glu_sub_pred pred_P so_None {{{ Γ, ℕ }}} {{{ A }}} SbΓℕ).
+  assert {{ EG Γ, ℕ, A ∈ glu_ctx_env pred_P (so_None::(so_Some sn)::anns) ↘ SbΓℕA }} by (invert_glu_rel_typ_unsorted HA; econstructor; mauto 4; try reflexivity).
   pose proof HM.
   invert_glu_rel_exp HM.
   pose proof HA.
   invert_glu_rel_typ_unsorted HA.
-  assert (forall Δ σ ρ, SbΓℕ Δ σ ρ -> glu_rel_typ_with_sub_unsorted pred_P None Δ A σ ρ) by mauto 3.
+  assert (forall Δ σ ρ, SbΓℕ Δ σ ρ -> glu_rel_typ_with_sub_unsorted pred_P so_None Δ A σ ρ) by mauto 3.
   (* eapply glu_rel_exp_implies_glu_rel_exp_unsorted. *)
   eexists; split; [eassumption |].
   intros.
@@ -1531,7 +1531,7 @@ Proof.
   inversion_clear_by_head (@nat_glu_exp_pred P).
   assert (glu_nat r Δ {{{ M[σ] }}} m) by mauto 2.
   assert {{ Δ ⊢s σ,,M[σ] ® ρ ↦ m ∈ SbΓℕ }} by (unfold SbΓℕ; mauto 3).
-  assert (glu_rel_typ_with_sub_unsorted pred_P None Δ A {{{ σ,,M[σ] }}} d{{{ ρ ↦ m }}}) by mauto 2.
+  assert (glu_rel_typ_with_sub_unsorted pred_P so_None Δ A {{{ σ,,M[σ] }}} d{{{ ρ ↦ m }}}) by mauto 2.
   inversion H12; subst.
 
   assert (exists r, {{ rec m ⟦return A | zero -> MZ | succ -> MS end⟧ ρ ↘ r }} /\ exp_rel Δ {{{ A[σ,, M[σ]] }}} {{{ rec M[σ] return A[q σ] | zero -> MZ[σ] | succ -> MS[q (q σ)] end }}} r) as [? []] by (eapply glu_rel_exp_natrec_helper; revgoals; mauto 4; econstructor; mauto 2).
@@ -1545,9 +1545,9 @@ Proof.
 Qed.
 
 Lemma glu_rel_exp_natrec {P} (pred_P : PredicativeSig P) : forall {sn so anns Γ A MZ MS M} {r : Ru_nat P sn},
-    {{ ⟪ pred_P ⟫ Γ, ℕ with (Some sn)::anns ⊩u A @ so }} ->
+    {{ ⟪ pred_P ⟫ Γ, ℕ with (so_Some sn)::anns ⊩u A @ so }} ->
     {{ ⟪ pred_P ⟫ Γ with anns ⊩u MZ : A[Id,,zero] @ so }} ->
-    {{ ⟪ pred_P ⟫ Γ, ℕ, A with so::(Some sn)::anns ⊩u MS : A[Wk∘Wk,,succ #1] @ so }} ->
+    {{ ⟪ pred_P ⟫ Γ, ℕ, A with so::(so_Some sn)::anns ⊩u MS : A[Wk∘Wk,,succ #1] @ so }} ->
     {{ ⟪ pred_P ⟫ Γ with anns ⊩ M : ℕ @ sn }} ->
     {{ ⟪ pred_P ⟫ Γ with anns ⊩u rec M return A | zero -> MZ | succ -> MS end : A[Id,,M] @ so }}.
 Proof.
